theories/LogicalRelation/Definition/Ne.v
@@ -15,22 +15,23 @@ Module neRedTy.
     `{WfType ta} `{ConvNeuConv ta} `{RedType ta}
     {Γ : context} {A B : term}
   : Set := {
+    nevar : neVar; 
     tyL : term;
     redL : [ Γ |- A :⤳*: tyL];
     tyR : term;
     redR : [ Γ |- B :⤳*: tyR];
-    eq : [ Γ |- tyL ~ tyR : U] ;
+    eq : [ Γ |- tyL ~ tyR : U |nevar] ;
   }.
 
   Arguments neRedTy {_ _ _ _}.
 
   Definition whredL `{GenericTypingProperties} {Γ : context} {A B : term} :
     neRedTy Γ A B -> [Γ |- A ↘ ].
-  Proof. intros []; econstructor; tea; constructor; now eapply convneu_whne. Defined.
+  Proof. intros []; econstructor; tea; econstructor; now eapply convneu_whne. Defined.
 
   Definition whredR `{GenericTypingProperties} {Γ : context} {A B : term} :
     neRedTy Γ A B -> [Γ |- B ↘ ].
-  Proof. intros []; econstructor; tea; constructor; eapply convneu_whne; now symmetry. Defined.
+  Proof. intros []; econstructor; tea; econstructor; eapply convneu_whne; now symmetry. Defined.
 
 End neRedTy.
 
@@ -59,18 +60,18 @@ Module neRedTmEq.
     termR     : term;
     redL      : [ Γ |- t :⤳*: termL : R.(neRedTy.tyL) ];
     redR      : [ Γ |- u :⤳*: termR : R.(neRedTy.tyL) ];
-    eq : [ Γ |- termL ~ termR : R.(neRedTy.tyL)] ;
+    eq : [ Γ |- termL ~ termR : R.(neRedTy.tyL) | R.(neRedTy.nevar)] ;
   }.
 
   Arguments neRedTmEq {_ _ _ _ _ _ _ _ _ _ _} _ _ _.
 
   Definition whredL `{GenericTypingProperties} {Γ : context} {t u A B : term} {R : [ Γ ||-ne A ≅ B]} :
     neRedTmEq R t u -> [Γ |- t ↘  R.(neRedTy.tyL)].
-  Proof.  intros []; econstructor; tea; constructor; now eapply convneu_whne. Defined.
+  Proof.  intros []; econstructor; tea; econstructor; now eapply convneu_whne. Defined.
 
   Definition whredR `{GenericTypingProperties} {Γ : context} {t u A B : term} {R : [ Γ ||-ne A ≅ B]} :
     neRedTmEq R t u -> [Γ |- u ↘  R.(neRedTy.tyL)].
-  Proof. intros []; econstructor; tea; constructor; eapply convneu_whne; now symmetry. Defined.
+  Proof. intros []; econstructor; tea; econstructor; eapply convneu_whne; now symmetry. Defined.
 
 
 End neRedTmEq.
@@ -85,40 +86,40 @@ Instance neRedTmWhRedTm `{GenericTypingProperties} {Γ A B} (R : [Γ ||-ne A ≅
   |}.
 Next Obligation.
   destruct h; cbn; eapply convtm_convneu; tea.
-  destruct R; cbn in *; constructor; now eapply convneu_whne.
+  destruct R; cbn in *; econstructor; now eapply convneu_whne.
 Qed.
 
 (** ** Reducibility of neutrals at an arbitrary type *)
 
 Module NeNf.
 
-  Record RedTmEq `{ta : tag} `{Typing ta} `{ConvNeuConv ta} {Γ A k l} : Set :=
+  Record RedTmEq `{ta : tag} `{Typing ta} `{ConvNeuConv ta} {Γ nevar A k l} : Set :=
     {
       tyL : [Γ |- k : A] ;
       tyR : [Γ |- l : A] ;
-      conv : [Γ |- k ~ l : A]
+      conv : [Γ |- k ~ l : A | nevar]
     }.
 
   Arguments RedTmEq {_ _ _}.
 
-  Definition whredL `{GenericTypingProperties} {Γ : context} {t u A : term} :
-    RedTmEq Γ A t u -> [Γ |- t ↘  A].
+  Definition whredL `{GenericTypingProperties} {Γ : context} {nevar} {t u A : term} :
+    RedTmEq Γ nevar A t u -> [Γ |- t ↘  A].
   Proof.
     intros []; econstructor.
     1: now eapply redtmwf_refl.
-    constructor; now eapply convneu_whne.
+    econstructor; now eapply convneu_whne.
   Defined.
 
-  Definition whredR `{GenericTypingProperties} {Γ : context} {t u A : term} :
-    RedTmEq Γ A t u -> [Γ |- u ↘  A].
+  Definition whredR `{GenericTypingProperties} {Γ : context} {nevar} {t u A : term} :
+    RedTmEq Γ nevar A t u -> [Γ |- u ↘  A].
   Proof.
     intros []; econstructor.
     1: now eapply redtmwf_refl.
-    constructor; eapply convneu_whne; now symmetry.
+    econstructor; eapply convneu_whne; now symmetry.
   Defined.
 
-  Definition conv_ `{GenericTypingProperties} {Γ : context} {t u A B : term} :
-    [Γ |- A ≅ B] -> RedTmEq Γ A t u -> RedTmEq Γ B t u.
+  Definition conv_ `{GenericTypingProperties} {Γ : context} {nevar} {t u A B : term} :
+    [Γ |- A ≅ B] -> RedTmEq Γ nevar A t u -> RedTmEq Γ nevar B t u.
   Proof.
     intros ? []; econstructor.
     1,2: now eapply ty_conv.
@@ -127,11 +128,11 @@ Module NeNf.
 
 End NeNf.
 
-Notation "[ Γ ||-NeNf k ≅ l : A ]" := (NeNf.RedTmEq Γ A k l) (at level 0, Γ, k, l, A at level 50).
+Notation "[ Γ ||-NeNf k ≅ l : A | nevar ]" := (NeNf.RedTmEq Γ nevar A k l) (at level 0, Γ, k, l, A at level 50).
 
 
 #[program]
-Instance NeNfWhRedTm `{GenericTypingProperties} {Γ A} (posA : isPosType A) : WhRedTmRel Γ A (NeNf.RedTmEq Γ A) :=
+Instance NeNfWhRedTm `{GenericTypingProperties} {Γ nevar A} (posA : isPosType A) : WhRedTmRel Γ A (NeNf.RedTmEq Γ nevar A) :=
   {| whredtmL := fun t u Rtu => NeNf.whredL Rtu ;
      whredtmR := fun t u Rtu => NeNf.whredR Rtu ;
   |}.
