theories/GenericTyping.v
@@ -412,7 +412,7 @@ Section GenericTyping.
       [ Γ,, ℓ |- P] ->
       [ Γ,, ℓt |- ht : term_decl P[tBox ℓ (tEval ℓt (tRel 0))]⇑ ] ->
       [ Γ,, ℓf |- hf : term_decl P[tBox ℓ (tEval ℓf (tRel 0))]⇑ ] ->
-      [ Γ |- n : ℓ] -> [Γ |- b : tBool] -> [Γ |- tApp (tEval ℓ n) (nat_to_term k) ≅ b] ->
+      [ Γ |- n : ℓ] -> [Γ |- b : tBool] -> [Γ |- tApp (tEval ℓ n) (nat_to_term k) ≅ b : tBool] ->
       [ Γ |- tEllElim k ℓ P ht hf n b : term_decl P[n..] ] ;
   }.
 
@@ -458,9 +458,9 @@ Section GenericTyping.
       [Γ |- t ⤳* t' : A] -> [Γ |- u ⤳* u' : A] ->
       [Γ |- A] -> [Γ |- t' : A] -> [Γ |- u' : A] ->
       [Γ |- A ≅ A] -> [Γ |- t' ≅ u' : A] -> [Γ |- t ≅ u : A] ;
-    convtm_convneu {Γ n n' A} :
+    convtm_convneu {Γ nevar n n' A} :
       isPosType A ->
-      [Γ |- n ~ n' : A] -> [Γ |- n ≅ n' : A] ;
+      [Γ |- n ~ n' : A | nevar ] -> [Γ |- n ≅ n' : A] ;
     convtm_prod {Γ A A' B B'} :
       [Γ |- A : U] ->
       [Γ |- A ≅ A' : U] -> [Γ,, A |- B ≅ B' : U] ->
@@ -551,55 +551,58 @@ Section GenericTyping.
       [ Γ,, ℓ |- P ≅ P' ] ->
       [ Γ,, ℓt |- ht ≅ ht' : term_decl P[tBox ℓ (tEval ℓt (tRel 0))]⇑ ] ->
       [ Γ,, ℓf |- hf ≅ hf' : term_decl P[tBox ℓ (tEval ℓf (tRel 0))]⇑ ] ->
-      [ Γ |- n ≅ n' : ℓ] -> [Γ |- b ≅ b' : tBool] -> [Γ |- tApp (tEval ℓ n) (nat_to_term k) ≅ b] ->
+      [ Γ |- n ≅ n' : ℓ] -> [Γ |- b ≅ b' : tBool] -> [Γ |- tApp (tEval ℓ n) (nat_to_term k) ≅ b : tBool] ->
       [ Γ |- tEllElim k ℓ P ht hf n b ≅ tEllElim k ℓ P' ht' hf' n' b' : term_decl P[n..] ] ;
   }.
 
   Class ConvNeuProperties :=
   {
     convneu_equiv {Γ A nevar} :: PER (conv_neu_ty nevar Γ A) ;
-    convneu_conv {Γ} {t u A A' : term} : [Γ |- t ~ u : A] -> [Γ |- A ≅ A'] -> [Γ |- t ~ u : A'] ;
-    convneu_wk {Γ Δ t u A} (ρ : Δ ≤ Γ) :
-      [|- Δ ] -> [Γ |- t ~ u : A] -> [Δ |- t⟨ρ⟩ ~ u⟨ρ⟩ : A⟨ρ⟩] ;
+    convneu_conv {Γ nevar} {t u A A' : term} : [Γ |- t ~ u : A | nevar ] -> [Γ |- A ≅ A'] -> [Γ |- t ~ u : A' | nevar ] ;
+    convneu_wk {Γ Δ t u A nevar} (ρ : Δ ≤ Γ) :
+      [|- Δ ] -> [Γ |- t ~ u : A | nevar ] -> [Δ |- t⟨ρ⟩ ~ u⟨ρ⟩ : A⟨ρ⟩ | nevar⟨ρ⟩ ] ;
     convneu_whne {Γ A t u nevar} : [Γ |- t ~ u : A | nevar ] -> whne nevar t;
     convneu_var {Γ n A} :
       [Γ |- tRel n : A] -> [Γ |- tRel n ~ tRel n : A] ;
-    convneu_app {Γ f g t u A B} :
-      [ Γ |- f ~ g : tProd A B ] ->
+    convneu_eval {Γ} {ℓ : ell} {v} {k : newnat ℓ} : [Γ |- tRel v : ell_decl ℓ] ->
+      [Γ |- tApp (tEval ℓ (tRel v)) (nat_to_term k) ~
+      tApp (tEval ℓ (tRel v)) (nat_to_term k) : tBool | ellNe k v];
+    convneu_app {Γ nevar f g t u A B} :
+      [ Γ |- f ~ g : tProd A B | nevar ] ->
       [ Γ |- t ≅ u : A ] ->
-      [ Γ |- tApp f t ~ tApp g u : term_decl B[t..] ] ;
-    convneu_natElim {Γ P P' hz hz' hs hs' n n'} :
+      [ Γ |- tApp f t ~ tApp g u : term_decl B[t..] | nevar ] ;
+    convneu_natElim {Γ nevar P P' hz hz' hs hs' n n'} :
         [Γ ,, tNat |- P ≅ P'] ->
         [Γ |- hz ≅ hz' : term_decl P[tZero..]] ->
         [Γ |- hs ≅ hs' : elimSuccHypTy' Γ P] ->
-        [Γ |- n ~ n' : tNat] ->
-        [Γ |- tNatElim P hz hs n ~ tNatElim P' hz' hs' n' : term_decl P[n..]] ;
-    convneu_boolElim {Γ P P' ht ht' hf hf' n n'} :
+        [Γ |- n ~ n' : tNat| nevar ] ->
+        [Γ |- tNatElim P hz hs n ~ tNatElim P' hz' hs' n' : term_decl P[n..]| nevar ] ;
+    convneu_boolElim {Γ nevar P P' ht ht' hf hf' n n'} :
         [Γ ,, tBool |- P ≅ P'] ->
         [Γ |- ht ≅ ht' : term_decl P[tTrue..]] ->
         [Γ |- hf ≅ hf' : term_decl P[tFalse..]] ->
-        [Γ |- n ~ n' : tBool] ->
-        [Γ |- tBoolElim P ht hf n ~ tBoolElim P' ht' hf' n' : term_decl P[n..]] ;
-    convneu_alpha {Γ : context} {i : list_index Γ} {t u n} :
-      [ Γ |- t ~ u : tNat ] ->
-      [ Γ |- tApp (tAlpha i) (nSucc n t) ~ tApp (tAlpha i) (nSucc n u) : tBool ];
-    convneu_emptyElim {Γ P P' e e'} :
+        [Γ |- n ~ n' : tBool| nevar ] ->
+        [Γ |- tBoolElim P ht hf n ~ tBoolElim P' ht' hf' n' : term_decl P[n..]| nevar ] ;
+    convneu_alpha {Γ : context} {i : list_index Γ} {t u n nevar} :
+      [ Γ |- t ~ u : tNat | nevar ] ->
+      [ Γ |- tApp (tAlpha i) (nSucc n t) ~ tApp (tAlpha i) (nSucc n u) : tBool | nevar ];
+    convneu_emptyElim {Γ nevar P P' e e'} :
         [Γ ,, tEmpty |- P ≅ P'] ->
-        [Γ |- e ~ e' : tEmpty] ->
-        [Γ |- tEmptyElim P e ~ tEmptyElim P' e' : term_decl P[e..]] ;
-    convneu_treeElim {Γ P P' hl hl' hn hn' t t'} :
+        [Γ |- e ~ e' : tEmpty | nevar ] ->
+        [Γ |- tEmptyElim P e ~ tEmptyElim P' e' : term_decl P[e..] | nevar ] ;
+    convneu_treeElim {Γ nevar P P' hl hl' hn hn' t t'} :
         [Γ ,, tTree |- P ≅ P'] ->
         [Γ |- hl ≅ hl' : elimLeafHypTy' Γ P] ->
         [Γ |- hn ≅ hn' : elimNodeHypTy' Γ P] ->
-        [Γ |- t ~ t' : tTree] ->
-        [Γ |- tTreeElim P hl hn t ~ tTreeElim P' hl' hn' t' : term_decl P[t..]] ;
-    convneu_fst {Γ A B p p'} :
-      [Γ |- p ~ p' : tSig A B] ->
-      [Γ |- tFst p ~ tFst p' : A] ;
-    convneu_snd {Γ A B p p'} :
-      [Γ |- p ~ p' : tSig A B] ->
-      [Γ |- tSnd p ~ tSnd p' : term_decl B[(tFst p)..]] ;
-    convneu_IdElim {Γ A A' x x' P P' hr hr' y y' e e'} :
+        [Γ |- t ~ t' : tTree | nevar ] ->
+        [Γ |- tTreeElim P hl hn t ~ tTreeElim P' hl' hn' t' : term_decl P[t..] | nevar ] ;
+    convneu_fst {Γ nevar A B p p'} :
+      [Γ |- p ~ p' : tSig A B | nevar ] ->
+      [Γ |- tFst p ~ tFst p' : A | nevar ] ;
+    convneu_snd {Γ nevar A B p p'} :
+      [Γ |- p ~ p' : tSig A B | nevar ] ->
+      [Γ |- tSnd p ~ tSnd p' : term_decl B[(tFst p)..] | nevar ] ;
+    convneu_IdElim {Γ nevar A A' x x' P P' hr hr' y y' e e'} :
       (* Parameters well formed: required by declarative instance *)
       [Γ |- A] ->
       [Γ |- x : A] ->
@@ -608,13 +611,27 @@ Section GenericTyping.
       [Γ ,, A ,, tId A⟨@wk1 Γ A⟩ x⟨@wk1 Γ A⟩ (tRel 0) |- P ≅ P'] ->
       [Γ |- hr ≅ hr' : term_decl P[tRefl A x .: x..]] ->
       [Γ |- y ≅ y' : A] ->
-      [Γ |- e ~ e' : tId A x y] ->
-      [Γ |- tIdElim A x P hr y e ~ tIdElim A' x' P' hr' y' e' : term_decl P[e .: y..]];
-    convneu_split {Γ t u A i new} :
+      [Γ |- e ~ e' : tId A x y | nevar ] ->
+      [Γ |- tIdElim A x P hr y e ~ tIdElim A' x' P' hr' y' e' : term_decl P[e .: y..] | nevar ];
+    convneu_split {Γ nevar t u A i new} :
       [|- Γ] ->
-      [ Γ,, i : new ↦ true |- t ~ u : A] ->
-      [ Γ,, i : new ↦ false |- t ~ u : A] ->
-      [ Γ |- t ~ u : A] ;
+      [ Γ,, i : new ↦ true |- t ~ u : A | nevar ] ->
+      [ Γ,, i : new ↦ false |- t ~ u : A | nevar ] ->
+      [ Γ |- t ~ u : A | nevar ] ;
+    convneu_xi nevar {Γ} {ℓ : ell} {m m' k} :
+      [Γ,, ℓ |- m ~ m' : tNat | nevar⟨@wk1 Γ ℓ⟩] ->
+      [Γ |- tXi ℓ (nSucc k m) ~ tXi ℓ (nSucc k m') : tTree | nevar] ;
+    convneu_xxi nevar {ℓ : ell} {Γ m m' n n' k} :
+      [Γ |- n ≅ n' : ℓ] ->
+      [Γ,, ℓ |- m ~ m' : tNat | nevar⟨@wk1 Γ ℓ⟩] ->
+      [Γ |- tXXi ℓ (nSucc k m) n ~ tXXi ℓ (nSucc k m') n' : tId tNat (dEval' Γ (tXi ℓ (nSucc k m)) (tEval ℓ n)) (nSucc k m)[n..] | nevar] ;
+    convneu_ellElim nevar {Γ ℓ k} {P P' ht ht' hf hf' n n' b b' : term} (ℓt := cons_ell ℓ k true) (ℓf := cons_ell ℓ k false):
+      [ Γ,, ℓ |- P ≅ P' ] ->
+      [ Γ,, ℓt |- ht ≅ ht' : term_decl P⟨wk_up ℓ (@wk1 Γ ℓt)⟩[(tBox ℓ (tEval ℓt (tRel 0)))..] ] ->
+      [ Γ,, ℓf |- hf ≅ hf' : term_decl P⟨wk_up ℓ (@wk1 Γ ℓf)⟩[(tBox ℓ (tEval ℓf (tRel 0)))..] ] ->
+      [ Γ |- n ≅ n' : ℓ] -> [Γ |- tApp (tEval ℓ n) (nat_to_term k) ≅ b : tBool] ->
+      [Γ |- b ~ b' : tBool | nevar] ->
+      [Γ |- tEllElim k ℓ P ht hf n b ~ tEllElim k ℓ P' ht' hf' n' b' : term_decl P[n..] | nevar];
   }.
 
   Class RedTypeProperties :=
@@ -759,6 +776,18 @@ Section GenericTyping.
       [Γ |- t ⤳* t : A] ;
     redtm_trans {Γ A} ::
       Transitive (red_tm Γ A) ;
+    redtm_ellElimTrue {Γ ℓ k} {P ht hf n : term} (ℓt := cons_ell ℓ k true) (ℓf := cons_ell ℓ k false):
+      [ Γ,, ℓ |- P] ->
+      [ Γ,, ℓt |- ht : term_decl P⟨wk_up ℓ (@wk1 Γ ℓt)⟩[(tBox ℓ (tEval ℓt (tRel 0)))..] ] ->
+      [ Γ,, ℓf |- hf : term_decl P⟨wk_up ℓ (@wk1 Γ ℓf)⟩[(tBox ℓ (tEval ℓf (tRel 0)))..] ] ->
+      [ Γ |- n : ℓ] -> [Γ |- tApp (tEval ℓ n) (nat_to_term k) ≅ tTrue : tBool] ->
+      [ Γ |- tEllElim k ℓ P ht hf n tTrue ⤳* ht[(tBox ℓt (tEval ℓ n))..] : P[n..]]; 
+    redtm_ellElimFalse {Γ ℓ k} {P ht hf n : term} (ℓt := cons_ell ℓ k true) (ℓf := cons_ell ℓ k false):
+      [ Γ,, ℓ |- P] ->
+      [ Γ,, ℓt |- ht : term_decl P⟨wk_up ℓ (@wk1 Γ ℓt)⟩[(tBox ℓ (tEval ℓt (tRel 0)))..] ] ->
+      [ Γ,, ℓf |- hf : term_decl P⟨wk_up ℓ (@wk1 Γ ℓf)⟩[(tBox ℓ (tEval ℓf (tRel 0)))..] ] ->
+      [ Γ |- n : ℓ] -> [Γ |- tApp (tEval ℓ n) (nat_to_term k) ≅ tFalse : tBool] ->
+      [ Γ |- tEllElim k ℓ P ht hf n tFalse ⤳* hf[(tBox ℓf (tEval ℓ n))..] : P[n..]]; 
   }.
 
 End GenericTyping.
@@ -899,6 +928,14 @@ Section GenericConsequences.
   `{!TypingProperties} `{!ConvTypeProperties}
   `{!ConvTermProperties} `{!ConvNeuProperties}
   `{!RedTypeProperties} `{!RedTermProperties}.
+
+
+  Lemma convneuvar_uniq {Γ nevarl nevarr nel ne ner A A'} : [Γ |- nel ~ ne : A | nevarl] -> [Γ |- ne ~ ner : A' | nevarr] -> nevarl = nevarr.
+  Proof.
+    intros hnel hner.
+    eapply nevar_uniq, convneu_whne, hner.
+    eapply convneu_whne, PER_Symmetric, hnel.
+  Qed.
 
   (** *** Meta-conversion *)
   (** Similar to conversion, but using a meta-level equality rather
@@ -1517,11 +1554,11 @@ Section GenericConsequences.
     rewrite wk_prod, wk_decl; gtyping.
   Qed.
 
-  Lemma convneu_app_ren {Γ Δ} {A f g a b dom cod : term} (ρ : Δ ≤ Γ) :
-    [Γ |- f ~ g : A] ->
+  Lemma convneu_app_ren {Γ Δ nevar} {A f g a b dom cod : term} (ρ : Δ ≤ Γ) :
+    [Γ |- f ~ g : A | nevar] ->
     [Γ |- A ≅ tProd dom cod] ->
     [Δ |- a ≅ b : term_decl dom⟨ρ⟩] ->
-    [Δ |- tApp f⟨ρ⟩ a ~ tApp g⟨ρ⟩ b : term_decl cod⟨wk_up dom ρ⟩[a ..]].
+    [Δ |- tApp f⟨ρ⟩ a ~ tApp g⟨ρ⟩ b : term_decl cod⟨wk_up dom ρ⟩[a ..] | nevar⟨ρ⟩].
   Proof.
     intros Hfg HA Hab.
     eapply convneu_app, Hab.
