theories/LogicalRelation/Definition/Empty.v
@@ -56,7 +56,8 @@ Section EmptyRedTmEq.
       nfR : term ;
       redL : [Γ |- t :⤳*: nfL : tEmpty] ;
       redR : [Γ |- u :⤳*: nfR : tEmpty ] ;
-      eq : [Γ ||-NeNf nfL ≅ nfR : tEmpty]
+      nevar : neVar;
+      eq : [Γ ||-NeNf nfL ≅ nfR : tEmpty | nevar]
   }.
   Arguments  EmptyRedTmEq : clear implicits.
 
@@ -66,12 +67,12 @@ Section EmptyRedTmEq.
 
     Definition whredL {Γ t u} : EmptyRedTmEq Γ t u -> [Γ |- t ↘ tEmpty].
     Proof.
-      intros []; econstructor; tea; unshelve eapply NeNf.whredL; cycle 3; tea.
+      intros []; econstructor; tea; unshelve eapply NeNf.whredL; cycle 4; tea.
     Defined.
 
     Definition whredR {Γ t u} : EmptyRedTmEq Γ t u -> [Γ |- u ↘ tEmpty].
     Proof.
-      intros []; econstructor; tea; unshelve eapply NeNf.whredR; cycle 3; tea.
+      intros []; econstructor; tea; unshelve eapply NeNf.whredR; cycle 4; tea.
     Defined.
   End  Def.
 
@@ -88,6 +89,6 @@ Instance EmptyRedTmEqWhRed `{GenericTypingProperties} {Γ} : WhRedTmRel Γ tEmpt
   {| whredtmL := fun t u Rtu => EmptyRedTmEq.whredL Rtu ;
     whredtmR := fun t u Rtu => EmptyRedTmEq.whredR Rtu |}.
 Next Obligation.
-  destruct h as [???? []].
-  eapply convtm_convneu; tea; constructor.
+  destruct h as [????? []].
+  eapply convtm_convneu; tea; econstructor.
 Qed.
