theories/LogicalRelation/Escape.v
@@ -66,7 +66,7 @@ Section Escapes.
       1-3: gtyping.
       2: now eapply urefl.
       eapply convtm_convneu; tea.
-      constructor; now eapply convneu_whne.
+      econstructor; now eapply convneu_whne.
     - intros ΠA ? [[] []]; cbn in *; prod_splitter.
       1,2: (eapply ty_conv; [gtyping|now symmetry]).
       destruct ΠA as [???? []]; cbn in *.
@@ -86,7 +86,7 @@ Section Escapes.
       1-3: gen_typing.
       2: now eapply urefl.
       tea.
-    - intros EA ? [???? []]; prod_splitter.
+    - intros EA ? [????? []]; prod_splitter.
       1,2: (eapply ty_conv; [gtyping|now symmetry]).
       destruct EA; eapply convtm_wfexp.
       1-3: gen_typing.
